Working on establishing the injection between global variables

x86/FlatAsmgenproof.v
@@ -2102,9 +2102,171 @@ Proof.
         rewrite Z.add_comm. setoid_rewrite DROP. auto. admit.
 
       * (** the head of gdefs is a global variable **)
+        monadInv TRANSG. destruct (gmap i) eqn:ILBL; try now inversion EQ.
+        destruct s. monadInv EQ. monadInv EQ2.
+        simpl in ALLOCG. 
+        destr_match_in ALLOCG; try now inversion ALLOCG.
+        destr_match_in EQ.
+        destr_match_in EQ; try now inversion EQ.
+        destr_match_in EQ; try now inversion EQ.
+        rename EQ2 into ALLOCINIT.
+        rename EQ3 into STOREZERO.
+        rename EQ4 into STOREINIT.
+        rename EQ into DROP.
+        exploit Mem.alloc_result; eauto using ALLOCINIT. intros.
+        exploit update_map_gmap_some; eauto. 
+        intros (slbl & GMAP & OFSRANGE).
+
+        (* alloc mapped injection *)
+        exploit (Mem.alloc_left_mapped_inject 
+                   (globs_meminj defs gmap) (def_frame_inj m1) m1 m1' 0 (init_data_list_size (gvar_init v)) m0
+                   b (gen_segblocks tprog (fst slbl)) (Ptrofs.unsigned (snd slbl))
+                   MINJ ALLOCINIT); eauto.
+        (* valid block *)
         admit.
+        (* valid offset *)
+        admit.
+        (* the offset of a location with permission is valid *)
+        admit.
+        (* preservation of permission *)
+        admit.
+        (* correct alignment *)
+        admit.
+        (* alloced memory has not been injected before *)
+        intros b0 delta' ofs k p GINJ PERM' OFSABSURD.
+        apply PERMS in PERM'. destruct PERM' as (id' & slbl' & FINDSYM' & GMAP' & OFS').
+        unfold globs_meminj in GINJ. apply Genv.find_invert_symbol in FINDSYM'.
+        rewrite FINDSYM' in GINJ. rewrite GMAP' in GINJ. inversion GINJ.
+        assert (fst slbl' = fst slbl).
+        { 
+          eapply gen_segblocks_injective; eauto. 
+          apply gen_segblocks_in_valid; eauto. 
+          eapply AGREE_SMINJ_INSTR.update_map_gmap_range; eauto.
+        }
+        apply Genv.invert_find_symbol in FINDSYM'.
+        exploit OFSRANGE; eauto. 
+        eapply partial_genv_find_symbol_inversion; eauto.
+        intros VALIDOFS. rewrite H2 in VALIDOFS. omega.
+        (* allocated memory is public *)
+        admit.
+        intros (f' & MINJ' & INJINCR & FNB & FINV).
+        erewrite alloc_pres_def_frame_inj in MINJ'; eauto.
+
+        (* normalize the resulting inject of alloc *)
+        assert (forall x, f' x = (globs_meminj (defs ++ (i, Some (Gvar v)) :: nil) gmap) x) as INJEQ.
+        {
+          intros x. destruct (eq_block x b).
+          (* x = b *)
+          subst x. unfold globs_meminj.
+          generalize (partial_genv_invert_symbol defs i (Some (Gvar v))).
+          intros INVSYM. subst b. rewrite BLOCKEQ. 
+          setoid_rewrite INVSYM. rewrite GMAP. rewrite <- BLOCKEQ. rewrite FNB.
+          auto.
+          (* x <> b *)
+          subst b. exploit FINV; eauto. intros FB. rewrite FB.
+          rewrite BLOCKEQ in n. unfold globs_meminj.
+          erewrite partial_genv_invert_symbol_pres; eauto.
+        }
+        exploit (Mem.inject_ext f' (globs_meminj (defs ++ (i, Some (Gvar v)) :: nil) gmap)); eauto.
+        intros MINJ''.
+
+        (* store_zeros injection *)
+
+        Lemma store_zeros_mapped_inject:
+          forall (f : meminj) (g : frameinj) (m1 : mem) (b1 : block) (lo hi : Z) 
+            (n1 m2 : mem) (b2 : block) (delta : Z),
+            Mem.inject f g m1 m2 ->
+            store_zeros m1 b1 lo hi = Some n1 ->
+            f b1 = Some (b2, delta) ->
+            exists n2 : mem, store_zeros m2  b2 (lo+delta) (hi+delta) = Some n2 /\ Mem.inject f g n1 n2.
+        Admitted.
+
+        exploit store_zeros_mapped_inject; eauto.
+        rewrite <- INJEQ. rewrite FNB. eauto.
+        intros (m2' & STOREZERO' & MINJZ).
         
-    + (* the head of gdefs is None *)
+        Lemma store_zeros_pres_def_frame_inj : forall m1 b lo hi m1',
+            store_zeros m1 b lo hi = Some m1' ->
+            def_frame_inj m1 = def_frame_inj m1'.
+        Admitted.
+
+        erewrite (store_zeros_pres_def_frame_inj m0) in MINJZ; eauto.
+        
+        (* store_init_data_list inject *)
+
+        Definition init_data_defined (d : AST.init_data) ids : Prop :=
+          match d with
+          | AST.Init_addrof id _ => In id ids
+          | _ => True
+          end.
+
+        Definition init_data_list_defined (l: list AST.init_data) ids : Prop :=
+          Forall (fun d => init_data_defined d ids) l.
+          
+        Lemma store_init_data_list_mapped_inject : forall defs gmap g m1 m1' m2 v v' b1 b2 delta ofs,
+            Mem.inject (globs_meminj defs gmap) g m1 m1' ->
+            init_data_list_defined (AST.gvar_init v) (map fst defs) ->
+            transl_gvar gmap v = OK v' -> 
+            (globs_meminj defs gmap) b1 = Some (b2, delta) ->
+            Genv.store_init_data_list ge m1 b1 ofs (gvar_init v) = Some m2 ->
+            exists m2', store_init_data_list tge m1' b2 (ofs+delta) (FlatAsmGlobdef.gvar_init unit v') = Some m2'
+                   /\ Mem.inject (globs_meminj defs gmap) g m2 m2'.
+        Admitted.
+
+        exploit store_init_data_list_mapped_inject; eauto. admit.
+        rewrite <- INJEQ. rewrite FNB. eauto.
+        intros (m3' & STOREINIT' & MINJSI).
+        
+        Lemma store_init_data_list_pres_def_frame_inj : forall m1 b1 ofs gv m1',
+            Genv.store_init_data_list ge m1 b1 ofs gv = Some m1' ->
+            def_frame_inj m1 = def_frame_inj m1'.
+        Admitted.
+
+        erewrite store_init_data_list_pres_def_frame_inj in MINJSI; eauto.
+        
+        (* dorp_perm inject *)
+        exploit Mem.drop_parallel_inject; eauto.
+        red. simpl. auto.
+        rewrite <- INJEQ. rewrite FNB. eauto.
+        intros (m4' & DROP' & MINJDR).
+        erewrite drop_perm_pres_def_frame_inj in MINJDR; eauto.
+        
+        (* apply the induction hypothesis *)
+        assert ((defs ++ (i, Some (Gvar v)) :: nil) ++ gdefs = AST.prog_defs prog) as DEFSTAIL'.
+        rewrite <- DEFSTAIL. rewrite <- app_assoc. simpl. auto.
+        exploit (IHgdefs x0 (defs ++ (i, Some (Gvar v)) :: nil) m); eauto using MINJDR, DEFSTAIL'.
+        (* nextblock *)
+        erewrite Mem.nextblock_drop; eauto.
+        erewrite Genv.store_init_data_list_nextblock; eauto.
+        erewrite Genv.store_zeros_nextblock; eauto.
+        erewrite Mem.nextblock_alloc; eauto. rewrite BLOCKEQ.      
+        rewrite partial_genv_next. auto.
+        (* perm *)
+        admit.
+        (* intros b0 ofs k p PERM'. *)
+        (* erewrite (drop_perm_perm _ _ _ _ _ _ EQ) in PERM'. destruct PERM' as [PERM' PIN]. *)
+        (* exploit Mem.perm_alloc_inv; eauto using ALLOCF. intros PERM1. *)
+        (* destruct eq_block.  *)
+        (* subst b0. exists i, slbl. split. rewrite partial_genv_find_symbol_eq. congruence.  *)
+        (* split; auto. omega. *)
+        (* apply PERMS in PERM1. destruct PERM1 as (id & slbl' & FINDSYM & GMAP' & OFS). *)
+        (* exists id, slbl'. split.        *)
+        (* rewrite <- DEFSTAIL in DEFNAMES. apply defs_names_distinct_not_in in DEFNAMES. *)
+        (* destruct (ident_eq i id).  *)
+        (* subst i. apply partial_genv_find_symbol_inversion in FINDSYM. congruence. *)
+        (* erewrite partial_genv_find_symbol_neq; eauto. *)
+        (* split; auto. *)
+        intros (m5' & ALLOCG' & FINALMINJ).
+        
+        (* Finish this case *)
+        admit.
+        (* exists m5'. split; auto. *)
+        (* simpl.  *)
+        (* rewrite GMAP in ILBL. inv ILBL. *)
+        (* unfold tge. repeat rewrite genv_gen_segblocks. setoid_rewrite Ptrofs.unsigned_repr. *)
+        (* rewrite Z.add_comm. setoid_rewrite DROP. auto. admit. *)
+        
+    + (* THE head of gdefs is None *)
       monadInv TRANSG. simpl in ALLOCG.
       set (mz := Mem.alloc m1 0 0) in *. destruct mz eqn:ALLOCZ. subst mz.
       eapply (IHgdefs tgdefs (defs ++ (i, None) :: nil)); eauto.
